Q1:
I can help you work through this integral! You're on the right track with integration by parts, but there's a small issue in your approach. Let me walk through the complete solution.

For $\int_0^\pi e^x \sin(x)\, dx$, we need to use integration by parts twice because both $e^x$ and $\sin(x)$ have simple derivatives and antiderivatives.

Let's use integration by parts: $\int u \, dv = uv - \int v \, du$

**First application:**
- Let $u = \sin(x)$, so $du = \cos(x) \, dx$
- Let $dv = e^x \, dx$, so $v = e^x$

This gives us:
$$\int e^x \sin(x) \, dx = e^x \sin(x) - \int e^x \cos(x) \, dx$$

**Second application** (for the remaining integral):
- Let $u = \cos(x)$, so $du = -\sin(x) \, dx$
- Let $dv = e^x \, dx$, so $v = e^x$

This gives us:
$$\int e^x \cos(x) \, dx = e^x \cos(x) - \int e^x(-\sin(x)) \, dx = e^x \cos(x) + \int e^x \sin(x) \, dx$$

Now substituting back:
$$\int e^x \sin(x) \, dx = e^x \sin(x) - [e^x \cos(x) + \int e^x \sin(x) \, dx]$$

$$\int e^x \sin(x) \, dx = e^x \sin(x) - e^x \cos(x) - \int e^x \sin(x) \, dx$$

Adding $\int e^x \sin(x) \, dx$ to both sides:
$$2\int e^x \sin(x) \, dx = e^x \sin(x) - e^x \cos(x) = e^x(\sin(x) - \cos(x))$$

Therefore:
$$\int e^x \sin(x) \, dx = \frac{e^x(\sin(x) - \cos(x))}{2}$$

**Now evaluating the definite integral:**
$$\int_0^\pi e^x \sin(x) \, dx = \left[\frac{e^x(\sin(x) - \cos(x))}{2}\right]_0^\pi$$

At $x = \pi$: $\sin(\pi) = 0$, $\cos(\pi) = -1$
At $x = 0$: $\sin(0) = 0$, $\cos(0) = 1$

$$= \frac{e^\pi(0 - (-1))}{2} - \frac{e^0(0 - 1)}{2} = \frac{e^\pi}{2} - \frac{-1}{2} = \frac{e^\pi + 1}{2}$$

So the correct answer is $\frac{e^\pi + 1}{2}$, not $1 + e^\pi$.

The key insight you were missing is that integration by parts needs to be applied twice for this type of integral, and you need to solve for the original integral algebraically when it reappears.
------------

Correctness:
Completeness:
Clarity:
Educational Value:
Tone/Coherence:

-----------

Q2:
I can see where you're getting confused! Let me walk through your reasoning and identify the issue.

Your approach of using the kinematic equation s = ut + ½at² is correct, and you're right to think about when the projectile returns to ground level (s = 0 vertically). However, there's a key distinction you're missing.

Let me break down what you did:
- You used the vertical motion equation: 0 = u_y·t - ½gt²
- Solving for t: t = 2u_y/g = 2v₀sin(30°)/g = 2(20)(0.5)/9.8 ≈ 2.04 s
- Then you calculated distance as u·t, which gives you about 81.5m

**The problem:** You're calculating the horizontal distance traveled, not the total distance. When you use "u·t", you're using the initial speed v₀ = 20 m/s, but the projectile doesn't travel in the direction of its initial velocity for the entire flight.

**What you should calculate:** The horizontal distance (range) is:
- Horizontal velocity: v_x = v₀cos(30°) = 20 × (√3/2) ≈ 17.32 m/s
- Horizontal distance: R = v_x × t = 17.32 × 2.04 ≈ 35.3 m

Since the slope has angle α = 0° (horizontal ground), the distance along the slope is simply the horizontal distance: **35.3 m**.

The 81.5m you calculated would be the distance if the projectile somehow maintained its initial velocity direction throughout the flight, which isn't what happens in projectile motion.

The key insight: in projectile motion, only the horizontal velocity component remains constant (ignoring air resistance), while the vertical component changes due to gravity.
------------

Correctness:
Completeness:
Clarity:
Educational Value:
Tone/Coherence:

-----------

Q3:
Let me check your work step by step.

First, let's identify the coefficients in the quadratic equation when k=0 and p=1:
$3x^2 + (p+3k)x - (p^2-3k) = 0$

When k=0 and p=1:
- $a = 3$
- $b = p + 3k = 1 + 3(0) = 1$
- $c = -(p^2 - 3k) = -(1^2 - 3(0)) = -1$

So the equation becomes: $3x^2 + x - 1 = 0$

Now using the quadratic formula: $x = \frac{-b \pm \sqrt{b^2 - 4ac}}{2a}$

$x = \frac{-1 \pm \sqrt{1^2 - 4(3)(-1)}}{2(3)}$

$x = \frac{-1 \pm \sqrt{1 + 12}}{6}$

$x = \frac{-1 \pm \sqrt{13}}{6}$

I notice you wrote "x = (-1+sqrt(1-(4)(3)(-1)))/6" but you seem to have made a small error in the discriminant calculation. You wrote "sqrt(1-(4)(3)(-1))" but it should be "sqrt(1**+**(4)(3)(1))" since $-4ac = -4(3)(-1) = +12$.

So the correct discriminant is $1 + 12 = 13$, which you did get right in your final answer.

Your final result $x = \frac{-1 + \sqrt{13}}{6}$ is correct for one of the roots (you found the positive root). The complete solution would be:

$x = \frac{-1 + \sqrt{13}}{6}$ or $x = \frac{-1 - \sqrt{13}}{6}$

So your calculation is essentially correct - you just had a minor notation issue in the middle step, but your final answer is right!
------------

Correctness:
Completeness:
Clarity:
Educational Value:
Tone/Coherence:

-----------

Q4:
I can see where you've gotten confused! There are a couple of issues with your approach that I'll help you work through.

**First issue: Ohm's Law**
You wrote Ohm's law as I = VR, but the correct formula is:
**I = V/R** (current equals voltage divided by resistance)

**Second issue: Current calculation**
When you calculated I₁ = 120A, I₂ = 240A, and I₃ = 180A, you used I = VR instead of I = V/R. Let's recalculate:

For parallel circuits, each resistor sees the same voltage (12V), so:
- I₁ = V/R₁ = 12V/10Ω = **1.2A**
- I₂ = V/R₂ = 12V/20Ω = **0.6A**  
- I₃ = V/R₃ = 12V/15Ω = **0.8A**

**Total current:**
In parallel circuits, currents add up:
I_total = I₁ + I₂ + I₃ = 1.2 + 0.6 + 0.8 = **2.6A**

**Equivalent resistance:**
You were on the right track with the parallel resistance formula. For resistors in parallel:
1/R_eq = 1/R₁ + 1/R₂ + 1/R₃
1/R_eq = 1/10 + 1/20 + 1/15
1/R_eq = 6/60 + 3/60 + 4/60 = 13/60
R_eq = 60/13 ≈ **4.62Ω**

**Check:** Using I = V/R_eq = 12V/(60/13)Ω = 12 × 13/60 = 2.6A ✓

So your equivalent resistance calculation was correct, but the total current should be 2.6A, not 55.4A. The key was fixing the Ohm's law formula!
------------

Correctness:
Completeness:
Clarity:
Educational Value:
Tone/Coherence:

-----------

Q5:
Looking at your solution, I need to point out that there's an issue with your approach. Let me work through this step-by-step to show you the correct method.

First, let's establish what we know:
- Square area = 8 m², so each side length = √8 = 2√2 m
- The sector has a 90° central angle
- Two vertices lie on the radii, two on the arc

The key insight is understanding the geometry. If we place the sector with its vertex at the origin and the two radii along the positive x and y axes, then due to symmetry, the square will be positioned at a 45° angle to these axes.

Let me set up coordinates. If the square has side length s = 2√2, and it's rotated 45° from the axes, then the distance from the center of the circle to any vertex on the arc can be found using the constraint that these vertices must lie on both the square and the circular arc.

For a square inscribed this way in a 90° sector, if we call the distance from the origin to a corner vertex d, then the geometry gives us:

The square's diagonal from center to corner vertex, when the square is at 45° to the radii, creates a specific relationship. The distance d must satisfy the constraint that the vertex lies on the circle of radius r.

Through the geometric relationship in this configuration:
d = s√2 = 2√2 × √2 = 4 meters

So your final answer of x = 4√2 ≈ 5.66 meters is incorrect. The correct distance is **4 meters**.

Your error was in the trigonometric relationship. The expression "x = A cos(45°)" doesn't correctly capture the geometric relationship in this problem. The actual relationship involves the square's orientation and how it fits within the sector, not a simple trigonometric function of the area.

The correct approach involves recognizing that for a square inscribed in a 90° sector with this specific orientation, the distance from center to corner vertex equals the square's side length times √2, which gives us exactly 4 meters.
------------

Correctness:
Completeness:
Clarity:
Educational Value:
Tone/Coherence:

-----------

Q6:
Let me check your working step by step.

First, let's clarify the setup: we have 5 blue balls, 3 red balls, 0 black balls (so 8 total), and we're drawing 3 balls without replacement. We want exactly 2 red balls.

Your approach has the right idea, but there's an important issue with the order and calculation:

**Your calculation:** 3/8 × 2/7 × 5/6

This calculates the probability of drawing red, then red, then blue in that specific order. However, there are multiple ways to get exactly 2 red balls out of 3 draws:
- Red, Red, Blue (RRB)
- Red, Blue, Red (RBR)  
- Blue, Red, Red (BRR)

**The correct approach:**

Method 1 - Count all orderings:
- P(RRB) = (3/8) × (2/7) × (5/6) = 30/336
- P(RBR) = (3/8) × (5/7) × (2/6) = 30/336
- P(BRR) = (5/8) × (3/7) × (2/6) = 30/336

Total probability = 30/336 + 30/336 + 30/336 = 90/336 = 15/56

Method 2 - Use combinations (hypergeometric distribution):
P = C(3,2) × C(5,1) / C(8,3) = 3 × 5 / 56 = 15/56

So your calculation gave you 30/336 = 5/84, but the correct answer is 15/56 = 45/252 = 15/84.

You were missing the factor of 3 because there are 3 different orders to arrange 2 red balls and 1 blue ball in 3 positions.
------------

Correctness:
Completeness:
Clarity:
Educational Value:
Tone/Coherence:

-----------