Q1:
Let's carefully evaluate the integral \( I = \int e^x \sin(x) \, dx \) using integration by parts (IBP). Then we'll compute the definite integral from \( x = \frac{\pi}{6} \) to \( x = \frac{3\pi}{4} \).

### Step 1: Integration by Parts
Recall IBP: \( \int u \, dv = uv - \int v \, du \).

Let:
- \( u = \sin(x) \), so \( du = \cos(x) \, dx \)
- \( dv = e^x \, dx \), so \( v = e^x \)

Apply IBP:
$$
\int e^x \sin(x) \, dx = \sin(x) \cdot e^x - \int e^x \cos(x) \, dx = e^x \sin(x) - \int e^x \cos(x) \, dx
$$

Now, apply IBP again to \( \int e^x \cos(x) \, dx \):
Let:
- \( u = \cos(x) \), so \( du = -\sin(x) \, dx \)
- \( dv = e^x \, dx \), so \( v = e^x \)

Then:
$$
\int e^x \cos(x) \, dx = \cos(x) \cdot e^x - \int e^x (-\sin(x)) \, dx = e^x \cos(x) + \int e^x \sin(x) \, dx
$$

Substitute back into the first equation:
$$
\int e^x \sin(x) \, dx = e^x \sin(x) - \left[ e^x \cos(x) + \int e^x \sin(x) \, dx \right]
$$
$$
= e^x \sin(x) - e^x \cos(x) - \int e^x \sin(x) \, dx
$$

Now, let \( I = \int e^x \sin(x) \, dx \). Then:
$$
I = e^x \sin(x) - e^x \cos(x) - I
$$
$$
2I = e^x \sin(x) - e^x \cos(x)
$$
$$
I = \frac{e^x (\sin(x) - \cos(x))}{2} + C
$$

So the general antiderivative is:
$$
F(x) = \frac{e^x (\sin(x) - \cos(x))}{2} + C
$$

### Step 2: Evaluate the Definite Integral from \( \frac{\pi}{6} \) to \( \frac{3\pi}{4} \)
We need:
$$
I = \int_{\pi/6}^{3\pi/4} e^x \sin(x) \, dx = F\left(\frac{3\pi}{4}\right) - F\left(\frac{\pi}{6}\right)
$$

Compute \( F\left(\frac{3\pi}{4}\right) \):
$$
\sin\left(\frac{3\pi}{4}\right) = \frac{\sqrt{2}}{2}, \quad \cos\left(\frac{3\pi}{4}\right) = -\frac{\sqrt{2}}{2}
$$
$$
F\left(\frac{3\pi}{4}\right) = \frac{e^{3\pi/4} \left( \frac{\sqrt{2}}{2} - \left(-\frac{\sqrt{2}}{2}\right) \right)}{2} = \frac{e^{3\pi/4} \left( \frac{\sqrt{2}}{2} + \frac{\sqrt{2}}{2} \right)}{2} = \frac{e^{3\pi/4} (\sqrt{2})}{2}
$$

Compute \( F\left(\frac{\pi}{6}\right) \):
$$
\sin\left(\frac{\pi}{6}\right) = \frac{1}{2}, \quad \cos\left(\frac{\pi}{6}\right) = \frac{\sqrt{3}}{2}
$$
$$
F\left(\frac{\pi}{6}\right) = \frac{e^{\pi/6} \left( \frac{1}{2} - \frac{\sqrt{3}}{2} \right)}{2} = \frac{e^{\pi/6} (1 - \sqrt{3})}{4}
$$

Therefore:
$$
I = \frac{e^{3\pi/4} \sqrt{2}}{2} - \frac{e^{\pi/6} (1 - \sqrt{3})}{4}
$$

### Step 3: Numerical Approximation
Let’s compute numerical values:
- \( e^{3\pi/4} \approx e^{2.3562} \approx 10.550 \)
- \( e^{\pi/6} \approx e^{0.5236} \approx 1.688 \)
- \( \sqrt{2} \approx 1.4142 \)
- \( \sqrt{3} \approx 1.732 \)

Then:
$$
F\left(\frac{3\pi}{4}\right) \approx \frac{10.550 \times 1.4142}{2} \approx \frac{14.92}{2} = 7.46
$$
$$
F\left(\frac{\pi}{6}\right) \approx \frac{1.688 \times (1 - 1.732)}{4} = \frac{1.688 \times (-0.732)}{4} \approx \frac{-1.236}{4} = -0.309
$$

So:
$$
I \approx 7.46 - (-0.309) = 7.769
$$

This is approximately 7.77, not 9.3.

### Step 4: Check Your Work
You mentioned:
> I choose dv/dx as e^x and u as sin(x), so that the integral on the first IBP was e^xcosx.

Actually, the first IBP gives:
$$
\int e^x \sin(x) \, dx = e^x \sin(x) - \int e^x \cos(x) \, dx
$$
So the next integral is \( \int e^x \cos(x) \, dx \), not \( e^x \cos(x) \).

Then you said:
> Since you get e^xsinx the next time round, you can rearrange and then get that F(x) = e^xsin(x)+e^xcos(x)+c.

This is incorrect. The correct rearrangement (as shown above) gives:
$$
I = e^x \sin(x) - e^x \cos(x) - I \implies 2I = e^x (\sin(x) - \cos(x)) \implies I = \frac{e^x (\sin(x) - \cos(x))}{2} + C
$$
Your result \( F(x) = e^x \sin(x) + e^x \cos(x) + C \) is wrong because it misses the factor of 1/2 and has a sign error.

### Conclusion:
Your teacher is correct to disagree. Your antiderivative is incorrect due to a sign error and missing factor. The correct antiderivative is \( \frac{e^x (\sin(x) - \cos(x))}{2} + C \), and the definite integral from \( \frac{\pi}{6} \) to \( \frac{3\pi}{4} \) is approximately 7.77, not 9.3.

**Final Answer:**
$$
\boxed{
\int e^x \sin(x) \, dx = \frac{e^x (\sin(x) - \cos(x))}{2} + C
}
$$
$$
\int_{\pi/6}^{3\pi/4} e^x \sin(x) \, dx = \frac{e^{3\pi/4} \sqrt{2}}{2} - \frac{e^{\pi/6} (1 - \sqrt{3})}{4} \approx 7.77
$$
------------

Correctness:
Completeness:
Clarity:
Educational Value:
Tone/Coherence:

-----------

Q2:
Let's carefully analyze the problem and your solution step by step.

**Given:**
- Initial speed \( v_0 = 20 \) m/s
- Launch angle \( \theta = 30^\circ \) above the horizontal
- Slope inclined at \( -\alpha \), meaning downward slope with \( \alpha = 15^\circ \) (so the slope is below the horizontal)
- No air resistance
- We need the distance along the slope to the first point of contact.

Your formula for the range along the slope is:
$$
R = \frac{2 v_0^2 \cos\theta \sin(\theta + \alpha)}{g \cos^2\alpha}
$$
Let's verify this formula.

**Derivation of the Range on an Inclined Plane:**
When a projectile is launched from a point on a slope inclined at angle \( \alpha \) (positive if upward, negative if downward), the range along the slope can be found by solving the equations of motion.

Set up coordinates:
- Let the launch point be at the origin.
- The slope is inclined at angle \( -\alpha \) (so downward). For convenience, we can define \( \alpha > 0 \) for the downward slope. So here \( \alpha = 15^\circ \).

The equations of motion:
$$
x = (v_0 \cos\theta) t
$$
$$
y = (v_0 \sin\theta) t - \frac{1}{2} g t^2
$$

The slope is defined by \( y = -(\tan\alpha) x \) (since downward slope).

The projectile hits the slope when:
$$
(v_0 \sin\theta) t - \frac{1}{2} g t^2 = -(\tan\alpha) (v_0 \cos\theta) t
$$
Solve for \( t \) (excluding \( t=0 \)):
$$
v_0 \sin\theta - \frac{1}{2} g t = -(\tan\alpha) v_0 \cos\theta
$$
$$
\frac{1}{2} g t = v_0 \sin\theta + v_0 \cos\theta \tan\alpha
$$
$$
t = \frac{2 v_0}{g} (\sin\theta + \cos\theta \tan\alpha)
$$

Now, the distance along the slope \( R \) is related to \( x \) and \( y \) by:
$$
R = \sqrt{x^2 + y^2} = \sqrt{x^2 + (\tan^2\alpha) x^2} = x \sqrt{1 + \tan^2\alpha} = \frac{x}{\cos\alpha}
$$
Since \( x = (v_0 \cos\theta) t \), we have:
$$
R = \frac{v_0 \cos\theta \, t}{\cos\alpha}
$$
Substitute \( t \):
$$
R = \frac{v_0 \cos\theta}{\cos\alpha} \cdot \frac{2 v_0}{g} (\sin\theta + \cos\theta \tan\alpha)
$$
$$
= \frac{2 v_0^2 \cos\theta}{g \cos\alpha} \left( \sin\theta + \cos\theta \cdot \frac{\sin\alpha}{\cos\alpha} \right)
$$
$$
= \frac{2 v_0^2 \cos\theta}{g \cos\alpha} \left( \frac{\sin\theta \cos\alpha + \cos\theta \sin\alpha}{\cos\alpha} \right)
$$
$$
= \frac{2 v_0^2 \cos\theta}{g \cos^2\alpha} \sin(\theta + \alpha)
$$
So your formula is correct:
$$
R = \frac{2 v_0^2 \cos\theta \sin(\theta + \alpha)}{g \cos^2\alpha}
$$

Now plug in the values:
- \( v_0 = 20 \) m/s
- \( \theta = 30^\circ \)
- \( \alpha = 15^\circ \)
- \( g = 9.8 \) m/s² (assuming standard gravity)

First, compute \( \theta + \alpha = 30^\circ + 15^\circ = 45^\circ \).

So:
$$
R = \frac{2 \times (20)^2 \times \cos(30^\circ) \times \sin(45^\circ)}{9.8 \times \cos^2(15^\circ)}
$$

Calculate step by step:
- \( v_0^2 = 400 \)
- \( \cos(30^\circ) = \frac{\sqrt{3}}{2} \approx 0.8660 \)
- \( \sin(45^\circ) = \frac{\sqrt{2}}{2} \approx 0.7071 \)
- \( \cos(15^\circ) \approx 0.9659 \), so \( \cos^2(15^\circ) \approx (0.9659)^2 = 0.9330 \)

Now numerator:
\( 2 \times 400 \times 0.8660 \times 0.7071 = 2 \times 400 \times 0.6124 = 2 \times 244.96 = 489.92 \)

Denominator:
\( 9.8 \times 0.9330 = 9.1434 \)

So:
\( R = \frac{489.92}{9.1434} \approx 53.58 \) m

Wait, this is much larger than your value of 2.68 m. I see you might have missed the \( v_0^2 \) in your formula? Your written formula has \( v_0 \) but it should be \( v_0^2 \). You wrote:
$$
R = \tfrac{2 v_0 \cos\theta \sin(\theta + \alpha)}{g \cos^2\alpha}
$$
but it should be:
$$
R = \tfrac{2 v_0^2 \cos\theta \sin(\theta + \alpha)}{g \cos^2\alpha}
$$
So you probably forgot the square on \( v_0 \).

With the correct formula, \( R \approx 53.58 \) m.

But let me double-check with exact calculation:

\( \cos(30^\circ) = \sqrt{3}/2 \)
\( \sin(45^\circ) = \sqrt{2}/2 \)
\( \cos(15^\circ) = \cos(45-30) = \cos45\cos30 + sin45\sin30 = (\sqrt{2}/2)(\sqrt{3}/2) + (\sqrt{2}/2)(1/2) = (\sqrt{6} + \sqrt{2})/4 \)

So \( \cos^2(15^\circ) = [(\sqrt{6} + \sqrt{2})/4]^2 = (6 + 2 + 2\sqrt{12})/16 = (8 + 4\sqrt{3})/16 = (2 + \sqrt{3})/4 \)

Now:
Numerator: \( 2 v_0^2 \cos\theta \sin(\theta+\alpha) = 2 \times 400 \times (\sqrt{3}/2) \times (\sqrt{2}/2) = 400 \times \sqrt{3} \times \sqrt{2} / 2 = 200 \sqrt{6} \)

Denominator: \( g \cos^2\alpha = 9.8 \times (2 + \sqrt{3})/4 \)

So:
\( R = \frac{200 \sqrt{6}}{9.8 \cdot (2 + \sqrt{3})/4} = \frac{200 \sqrt{6} \cdot 4}{9.8 (2 + \sqrt{3})} = \frac{800 \sqrt{6}}{9.8 (2 + \sqrt{3})} \)

Now \( \sqrt{6} \approx 2.4495 \), \( \sqrt{3} \approx 1.732 \), so \( 2 + 1.732 = 3.732 \)

So numerator: \( 800 \times 2.4495 = 1959.6 \)
Denominator: \( 9.8 \times 3.732 = 36.5736 \)
\( R = 1959.6 / 36.5736 \approx 53.58 \) m

So the correct range along the slope is about 53.58 meters.

**Why you got 2.68 m?**
You probably used \( v_0 \) instead of \( v_0^2 \). If we use your formula without the square:
\( R = \frac{2 \times 20 \times \cos30 \times \sin45}{9.8 \times \cos^2 15} = \frac{40 \times 0.8660 \times 0.7071}{9.8 \times 0.9330} = \frac{24.49}{9.1434} \approx 2.68 \) m

So indeed, you missed the square on \( v_0 \).

**Conclusion:**
Your formula is correct, but you made a calculation error by using \( v_0 \) instead of \( v_0^2 \). The correct distance along the slope is approximately 53.58 meters.

You should ask your teacher to reconsider, acknowledging that you forgot the square on \( v_0 \) in your calculation, but the formula itself is correct.

**Final Answer:**
$$
\boxed{53.6\ \text{m}}
$$
(rounded to one decimal place)
------------

Correctness:
Completeness:
Clarity:
Educational Value:
Tone/Coherence:

-----------

Q3:
Let's carefully go through the problem step by step to understand what might have happened.

**Original equation:**
$$
3x^2 + (p + 3k)x - (p^2 - 3k) = 0
$$

**Given:**
- \( k = 1 \)
- \( p = 2 \)

**Substitute \( k = 1 \) and \( p = 2 \):**
1. Coefficient of \(x\): \(p + 3k = 2 + 3(1) = 2 + 3 = 5\)
2. Constant term: \(-(p^2 - 3k) = -( (2)^2 - 3(1) ) = -(4 - 3) = -(1) = -1\)

So the equation becomes:
$$
3x^2 + 5x - 1 = 0
$$

**Solve using the quadratic formula:**
$$
x = \frac{-b \pm \sqrt{b^2 - 4ac}}{2a}
$$
where \(a = 3\), \(b = 5\), \(c = -1\).

Discriminant:
$$
D = b^2 - 4ac = (5)^2 - 4(3)(-1) = 25 + 12 = 37
$$

So the roots are:
$$
x = \frac{-5 \pm \sqrt{37}}{6}
$$

**Your calculation:**
You computed:
$$
(-5 \pm \sqrt{5^2 - 4(3)(1)}) / (2 \cdot 3) = (-5 \pm \sqrt{25 - 12}) / 6 = (-5 \pm \sqrt{13}) / 6
$$

**Mistake:**
You used \(c = 1\) instead of \(c = -1\). Specifically:
- In the discriminant, you computed \(4ac = 4(3)(1) = 12\), but it should be \(4(3)(-1) = -12\).
- Therefore, \(b^2 - 4ac = 25 - (-12) = 25 + 12 = 37\), not \(25 - 12 = 13\).

So the correct discriminant is \(37\), not \(13\).

**Correct roots:**
$$
x = \frac{-5 \pm \sqrt{37}}{6}
$$

**Why you were marked wrong:**
You made an error in the sign of the constant term when computing the discriminant. The constant term \(c\) is \(-1\), not \(1\). Therefore, your discriminant was incorrect, leading to wrong roots.

**Summary:**
- Correct equation after substitution: \(3x^2 + 5x - 1 = 0\)
- Correct discriminant: \(D = 5^2 - 4(3)(-1) = 25 + 12 = 37\)
- Correct roots: \(x = \frac{-5 \pm \sqrt{37}}{6}\)

You should have:
$$
x = \frac{-5 \pm \sqrt{37}}{6}
$$
not
$$
x = \frac{-5 \pm \sqrt{13}}{6}
$$

This is likely why your teacher marked it wrong. Always double-check the signs when substituting values, especially when negatives are involved.
------------

Correctness:
Completeness:
Clarity:
Educational Value:
Tone/Coherence:

-----------

Q4:
Let's carefully analyze the problem step by step to determine if your solution is correct.

**Given:**
- Supply voltage \( V = 12  \text{V} \)
- Three resistors \( R_1, R_2, R_3 \) in parallel.
- \( R_1 = 10  \Omega \), \( R_2 = 20  \Omega \)
- Condition: \( I_1 + I_2 = I_3 \)

**Recall:**
For resistors in parallel, the voltage across each is the same (12 V). The current through each resistor is given by Ohm's law:
- \( I_1 = \frac{V}{R_1} = \frac{12}{10} = 1.2  \text{A} \)
- \( I_2 = \frac{V}{R_2} = \frac{12}{20} = 0.6  \text{A} \)
- \( I_3 = \frac{V}{R_3} = \frac{12}{R_3} \)

**Condition:**
$$
I_1 + I_2 = I_3
$$
Substitute the known values:
$$
1.2 + 0.6 = \frac{12}{R_3}
$$
$$
1.8 = \frac{12}{R_3}
$$
Solve for \( R_3 \):
$$
R_3 = \frac{12}{1.8} = \frac{120}{18} = \frac{20}{3} \approx 6.667  \Omega
$$

**Your approach:**
You calculated the equivalent resistance of \( R_1 \) and \( R_2 \) as \( \frac{20}{3}  \Omega \). Then you found the total current through these two as:
$$
I_{12} = \frac{V}{R_{12}} = \frac{12}{20/3} = 12 \times \frac{3}{20} = 1.8  \text{A}
$$
This is indeed \( I_1 + I_2 = 1.8  \text{A} \).

Then you set \( I_3 = 1.8  \text{A} \), so:
$$
\frac{12}{R_3} = 1.8
$$
$$
R_3 = \frac{12}{1.8} = \frac{20}{3}  \Omega
$$

This matches the calculation above.

**Why did you get \( R_3 = 0.15  \Omega \)?**
You wrote:
> 12/(3/20) = 80A

But note: \( \frac{12}{20/3} = 12 \times \frac{3}{20} = \frac{36}{20} = 1.8  \text{A} \), not 80 A. It seems you might have miscomputed:
- \( \frac{12}{3/20} = 12 \times \frac{20}{3} = 80  \text{A} \) is incorrect because the equivalent resistance is \( \frac{20}{3} \), not \( \frac{3}{20} \).

So your error was in inverting the fraction: you used \( \frac{3}{20} \) instead of \( \frac{20}{3} \).

**Conclusion:**
The correct value for \( R_3 \) is \( \frac{20}{3}  \Omega \approx 6.667  \Omega \).
Your method was correct in principle, but you made a calculation mistake when computing the current through \( R_1 \) and \( R_2 \). You should have found \( I_1 + I_2 = 1.8  \text{A} \), not 80 A.

Therefore, your teacher was right to mark it down due to the numerical error, but the approach was valid. The correct answer is \( R_3 = \frac{20}{3}  \Omega \).

**Final Answer:**
$$
\boxed{R_3 = \dfrac{20}{3}  \Omega \approx 6.667  \Omega}
$$
------------

Correctness:
Completeness:
Clarity:
Educational Value:
Tone/Coherence:

-----------

Q5:
Let's analyze the problem step by step to determine the correct area of the inscribed square.

**Given:**
- A circular sector (quadrant) with radius \( r = 10 \) and central angle \( \theta = 90^\circ \).
- A square is inscribed such that two vertices lie on the two radii (the perpendicular boundaries of the quadrant) and the other two lie on the arc.

**Your approach:**
You assumed that the square is oriented at \(45^\circ\) to the radii, and you concluded that the distance from the center to the point where the square touches the arc is \(x = r/2 = 5\). Then, you computed the side length as \(a = 2x \cos 45^\circ = 2 \cdot 5 \cdot \frac{\sqrt{2}}{2} = 5\sqrt{2}\), and the area as \(a^2 = (5\sqrt{2})^2 = 50\).

However, this assumption is incorrect. The square is not necessarily oriented at \(45^\circ\) to the radii. In fact, the orientation is determined by the condition that two vertices lie on the arc (which is curved) and two on the radii (which are straight). Therefore, we need to derive the correct orientation and side length.

**Correct approach:**

Let the square have side length \(a\). Place the center of the quadrant at \(O = (0,0)\). The two radii are along the positive \(x\)-axis and positive \(y\)-axis.

Let the square be positioned such that:
- One vertex lies on the \(x\)-axis: call it \(A = (x_1, 0)\).
- One vertex lies on the \(y\)-axis: call it \(B = (0, y_1)\).
- The other two vertices lie on the arc: call them \(C\) and \(D\).

Since it is a square, the sides are of length \(a\), and the diagonals are at \(45^\circ\) to the sides. However, the orientation of the square relative to the axes is not necessarily \(45^\circ\).

Let the square be oriented such that the side from \(A\) to \(D\) makes an angle \(\phi\) with the horizontal. Then:
- \(A = (x_1, 0)\).
- \(D = A + a(\cos\phi, \sin\phi) = (x_1 + a\cos\phi, a\sin\phi)\).
- \(B = A + a(-\sin\phi, \cos\phi) = (x_1 - a\sin\phi, a\cos\phi)\). But \(B\) lies on the \(y\)-axis, so its \(x\)-coordinate is 0: \(x_1 - a\sin\phi = 0 \implies x_1 = a\sin\phi\).
Also, \(B\) has \(y\)-coordinate \(y_1 = a\cos\phi\).

Now, \(D\) lies on the arc, so its distance from \(O\) is \(r = 10\):
$$
(x_1 + a\cos\phi)^2 + (a\sin\phi)^2 = 100.
$$
Substitute \(x_1 = a\sin\phi\):
$$
(a\sin\phi + a\cos\phi)^2 + (a\sin\phi)^2 = 100 \\
a^2 (\sin\phi + \cos\phi)^2 + a^2 \sin^2\phi = 100 \\
a^2 [ (\sin^2\phi + 2\sin\phi\cos\phi + \cos^2\phi) + \sin^2\phi ] = 100 \\
a^2 [ 1 + 2\sin\phi\cos\phi + \sin^2\phi ] = 100.
$$
Similarly, the other vertex on the arc (say \(C\)) should also satisfy the same condition, but it will yield a similar equation.

Alternatively, we can use symmetry: since the quadrant is symmetric about \(y=x\), the square should also be symmetric. This implies that the square is oriented at \(45^\circ\) to the axes? Actually, no: if the square were symmetric with respect to \(y=x\), then the vertex on the \(x\)-axis and the vertex on the \(y\)-axis should be symmetric, meaning \(x_1 = y_1\). From above, \(x_1 = a\sin\phi\) and \(y_1 = a\cos\phi\), so for \(x_1 = y_1\), we need \(\sin\phi = \cos\phi \implies \phi = 45^\circ\).

So indeed, by symmetry, the square is oriented at \(45^\circ\) to the axes. Therefore, \(\phi = 45^\circ\).

Then:
\(x_1 = a \sin 45^\circ = a \frac{\sqrt{2}}{2}\),
\(y_1 = a \cos 45^\circ = a \frac{\sqrt{2}}{2}\).

Now, vertex \(D\) (which is adjacent to \(A\) and \(B\)) has coordinates:
\(D = (x_1 + a\cos\phi, a\sin\phi) = \left( a\frac{\sqrt{2}}{2} + a\frac{\sqrt{2}}{2}, a\frac{\sqrt{2}}{2} \right) = (a\sqrt{2}, a\frac{\sqrt{2}}{2})\).

Its distance from \(O\) is \(r = 10\):
$$
(a\sqrt{2})^2 + \left( a\frac{\sqrt{2}}{2} \right)^2 = 100 \\
2a^2 + \frac{2a^2}{4} = 100 \\
2a^2 + \frac{a^2}{2} = 100 \\
\frac{4a^2 + a^2}{2} = 100 \\
\frac{5a^2}{2} = 100 \\
5a^2 = 200 \\
a^2 = 40.
$$
So the area of the square is \(a^2 = 40\).

**Verification:**
The vertex \(D\) is at \((a\sqrt{2}, a\frac{\sqrt{2}}{2}) = (\sqrt{80}, \sqrt{20}) = (4\sqrt{5}, 2\sqrt{5})\).
Its distance from origin: \(\sqrt{(4\sqrt{5})^2 + (2\sqrt{5})^2} = \sqrt{80 + 20} = \sqrt{100} = 10\), which is correct.

Similarly, the other vertex on the arc will also be at distance 10.

Therefore, the correct area is \(40\).

**Why your approach was incorrect:**
You assumed that the distance from the center to the point where the square touches the arc is \(r/2 = 5\). However, from the correct solution, the vertex \(D\) has \(x\)-coordinate \(a\sqrt{2} = \sqrt{40}\cdot \sqrt{2} = \sqrt{80} \approx 8.94\), and \(y\)-coordinate \(a\frac{\sqrt{2}}{2} \approx \sqrt{40} \cdot 0.707 \approx 4.47\), so its distance is 10, but its projection is not 5. Your assumption that the square is oriented at \(45^\circ\) to the radii is correct (by symmetry), but the relation you used (\(x = r/2\)) is not valid.

**Correct answer:**
$$
\boxed{40}
$$
The area of the inscribed square is 40 square units.
------------

Correctness:
Completeness:
Clarity:
Educational Value:
Tone/Coherence:

-----------

Q6:
Let's carefully analyze the problem and your solution step by step.

**Problem Recap:**
- Total balls: \( n = 7 \) blue, \( m = 5 \) red, \( k = 4 \) black. So total balls = \( 7 + 5 + 4 = 16 \).
- We draw \( r = 4 \) balls without replacement.
- We want the probability that exactly \( q = 3 \) of them are red.

**Your Approach:**
You computed:
$$
\binom{4}{3} \times \left( \frac{5}{12} \times \frac{4}{11} \times \frac{3}{10} \times \frac{7}{9} \right)
$$
Let's break this down:
- \(\binom{4}{3}\): This is the number of ways to choose which 3 of the 4 draws are red. This is correct.
- \(\frac{5}{12}\): Probability that the first ball drawn is red? But wait: total balls initially are 16, not 12. You used 12, which is the sum of red and blue (ignoring black). This is a mistake.

**Why is using 12 incorrect?**
The black balls are part of the total. When drawing without replacement, every ball (blue, red, black) has a chance to be drawn. By using 12 (which is only red + blue), you are effectively ignoring the black balls. This is wrong because:
- The probability of drawing a red ball on the first draw is \( \frac{5}{16} \), not \( \frac{5}{12} \).
- Similarly, the probability of drawing a blue ball is \( \frac{7}{16} \), but if you are ignoring black, you are overestimating the probabilities for red and blue.

**Correct Approach:**
We need exactly 3 red balls in 4 draws. The other ball must be non-red (i.e., blue or black). So the number of non-red balls is \( 7 + 4 = 11 \).

The probability can be computed using combinations (which is straightforward for such problems):
$$
P = \frac{\binom{5}{3} \binom{11}{1}}{\binom{16}{4}}
$$
Here:
- \(\binom{5}{3}\): ways to choose 3 red balls from 5.
- \(\binom{11}{1}\): ways to choose 1 non-red ball from 11 (7 blue + 4 black).
- \(\binom{16}{4}\): total ways to choose 4 balls from 16.

Now compute:
$$
\binom{5}{3} = 10, \quad \binom{11}{1} = 11, \quad \binom{16}{4} = \frac{16 \times 15 \times 14 \times 13}{4 \times 3 \times 2 \times 1} = 1820
$$
So,
$$
P = \frac{10 \times 11}{1820} = \frac{110}{1820} = \frac{11}{182}
$$
Simplify: divide numerator and denominator by 2? But 11 is prime and doesn't divide 182? Actually, 182 ÷ 11 = 16.545? Wait, let's check: 11 × 16 = 176, 182 - 176 = 6, so no. Alternatively, divide by 2: \( \frac{11}{182} = \frac{11}{2 \times 91} = \frac{11}{2 \times 7 \times 13} \), so it's already simplified. But wait, 110 and 1820 both divisible by 10? Actually, 110/1820 = 11/182 after dividing by 10.

Alternatively, we can compute step by step without combinations (using your sequential approach but correctly):

Probability of getting exactly 3 red and 1 non-red in a specific order (say first three red, then non-red):
$$
\frac{5}{16} \times \frac{4}{15} \times \frac{3}{14} \times \frac{11}{13}
$$
But there are \(\binom{4}{3} = 4\) orders (the non-red can be in any of the 4 positions). So total probability:
$$
4 \times \left( \frac{5}{16} \times \frac{4}{15} \times \frac{3}{14} \times \frac{11}{13} \right)
$$
Compute step by step:
- Numerator: \(4 \times 5 \times 4 \times 3 \times 11 = 4 \times 660 = 2640\)
- Denominator: \(16 \times 15 \times 14 \times 13 = 43680\)
So \(P = \frac{2640}{43680} = \frac{264}{4368} = \frac{33}{546} = \frac{11}{182}\), same as above.

**Your Calculation:**
You computed:
$$
\binom{4}{3} \times \left( \frac{5}{12} \times \frac{4}{11} \times \frac{3}{10} \times \frac{7}{9} \right) = 4 \times \left( \frac{5}{12} \times \frac{4}{11} \times \frac{3}{10} \times \frac{7}{9} \right)
$$
Compute inside:
\(5 \times 4 \times 3 \times 7 = 420\)
\(12 \times 11 \times 10 \times 9 = 11880\)
So \(4 \times \frac{420}{11880} = \frac{1680}{11880} = \frac{168}{1188} = \frac{14}{99}\) after simplifying (divide by 12: 168/12=14, 1188/12=99).

So you got \(\frac{14}{99}\), which is approximately 0.1414, while the correct probability is \(\frac{11}{182} \approx 0.06044\). So your answer is more than double the correct probability.

**Why did you get 14/99?**
Because you used a total of 12 (ignoring black balls) instead of 16. This effectively assumes that only red and blue balls are present, which is not true. By ignoring the black balls, you are increasing the probabilities for red and blue draws. For example:
- Probability of red on first draw: actually 5/16 ≈ 0.3125, but you used 5/12 ≈ 0.4167.
- Similarly, after drawing one red, probability of next red: actually 4/15 ≈ 0.2667, but you used 4/11 ≈ 0.3636.
So each step is overestimated.

**Conclusion:**
Your teacher is correct to mark you wrong. The error is in using a total of 12 (red+blue) instead of the actual total of 16 (including black). The black balls must be accounted for in the denominator.

**Correct Answer:**
$$
\boxed{\dfrac{11}{182}}
$$
------------

Correctness:
Completeness:
Clarity:
Educational Value:
Tone/Coherence:

-----------
