Q1:
<span style="color:Yellow">Let's evaluate the integral step by step</span>: <Tn> [1]

$$
I = \int_0^\pi e^x \sin(x)  dx
$$

We can use integration by parts. <span style="color:green">Recall the formula</span>: <Cl> [2]

$$
\int u  dv = uv - \int v  du
$$

Let:
$$
u = \sin(x) \quad \Rightarrow \quad du = \cos(x)  dx
$$
$$
dv = e^x  dx \quad \Rightarrow \quad v = e^x
$$

Apply integration by parts:

$$
I = \int e^x \sin(x)  dx = \sin(x) \cdot e^x - \int e^x \cos(x)  dx
$$

Now, we need to evaluate \(\int e^x \cos(x)  dx\). Apply integration by parts again:

Let:
$$
u = \cos(x) \quad \Rightarrow \quad du = -\sin(x)  dx
$$
$$
dv = e^x  dx \quad \Rightarrow \quad v = e^x
$$

So,
$$
\int e^x \cos(x)  dx = \cos(x) \cdot e^x - \int e^x (-\sin(x))  dx = e^x \cos(x) + \int e^x \sin(x)  dx
$$

Notice that \(\int e^x \sin(x)  dx = I\). Substitute back:

$$
I = e^x \sin(x) - \left[ e^x \cos(x) + I \right]
$$

Simplify:

$$
I = e^x \sin(x) - e^x \cos(x) - I
$$

Bring \(I\) to the left:

$$
I + I = e^x \sin(x) - e^x \cos(x)
$$
$$
2I = e^x (\sin(x) - \cos(x))
$$
$$
I = \frac{e^x}{2} (\sin(x) - \cos(x)) + C
$$

Now, evaluate the definite integral from \(0\) to \(\pi\):

$$
I = \left[ \frac{e^x}{2} (\sin(x) - \cos(x)) \right]_0^\pi
$$

At \(x = \pi\):
$$
\sin(\pi) = 0, \quad \cos(\pi) = -1
$$
$$
\frac{e^\pi}{2} (0 - (-1)) = \frac{e^\pi}{2} (1) = \frac{e^\pi}{2}
$$

At \(x = 0\):
$$
\sin(0) = 0, \quad \cos(0) = 1
$$
$$
\frac{e^0}{2} (0 - 1) = \frac{1}{2} (-1) = -\frac{1}{2}
$$

So,
$$
I = \frac{e^\pi}{2} - \left( -\frac{1}{2} \right) = \frac{e^\pi}{2} + \frac{1}{2} = \frac{e^\pi + 1}{2}
$$

Therefore, the value of the integral is:

$$
\boxed{\frac{e^\pi + 1}{2}}
$$

**Where you slipped up:**
You mentioned that you got \(1 + e^\pi\). This suggests you might have integrated incorrectly. Specifically, <span style="color:green">integrating \(e^x \sin(x)\) directly as \(-e^x \cos(x)\) is not correct because the derivative of \(-e^x \cos(x)\) is \(e^x \sin(x) - e^x \cos(x)\) (by the product rule), which is not the same as \(e^x \sin(x)\).</span> Hence, you missed the term involving \(\cos(x)\). The correct approach requires integration by parts twice to account for both the sine and exponential functions. [3]

------------
[1] - Neutral tone; not necessarily appropriate for the user.

[2] - Useful clarity; user appropriate

[3] - Educational value well provided; explaining the reasoning thoroughly behind the student's mistake. 

Correctness: 2 <!--Solution is fully correct-->

Completeness: 2 <!--Thorough reasoning is provided; appropriate for the student.-->

Clarity: 2 <!--Explanation of the solution is easy to follow, doesn't over explain the problem-->

Educational Value: 1 <!-- Mistake is well explained in the 'Where you slipped up section', however little technique or transferable advice is given.-->

Tone/Coherence: 1 <!-- Neutral Tone-->

#### Total: 8  <!--Response is well done, but lacks in empathy, general takaways or diagnostic advice-->
-----------

Q2:
Let's break down the problem step by step to identify where the reasoning might have gone astray.

**Given:**
- Initial speed \( v_0 = 20 \) m/s
- Launch angle \( \theta = 30^\circ \) above the horizontal
- Slope inclined at \( -\alpha \), but here \( \alpha = 0^\circ \), meaning the slope is horizontal (i.e., flat ground).
- No air resistance.

<span style="color:green">So, effectively, we have a projectile launched on flat ground. We need to find the horizontal distance traveled (range) before it hits the ground.</span> <Cl> <Cm> [1]

**Your reasoning:**
You used the vertical motion equation: \( s_y = u_y t + \frac{1}{2} a_y t^2 \).
At the point of impact, \( s_y = 0 \) (since it returns to the same vertical level).
So, \( 0 = (v_0 \sin \theta) t - \frac{1}{2} g t^2 \).
Solving for \( t \): \( t (v_0 \sin \theta - \frac{1}{2} g t) = 0 \), so non-zero solution is \( t = \frac{2 v_0 \sin \theta}{g} \).

Then, you calculated the distance as \( u \times t \), where \( u \) <span style="color:()">is presumably the horizontal velocity \( v_0 \cos \theta \).</span> <Cl> [2]
So, range \( R = (v_0 \cos \theta) \times t = (v_0 \cos \theta) \times \frac{2 v_0 \sin \theta}{g} = \frac{2 v_0^2 \sin \theta \cos \theta}{g} \).

Plugging in numbers:
\( v_0 = 20 \) m/s, \( \theta = 30^\circ \), \( g = 9.8 \) m/sÂ² (assuming standard value).
So, \( \sin 30^\circ = 0.5 \), \( \cos 30^\circ \approx 0.8660 \).
Then, \( R = \frac{2 \times (20)^2 \times 0.5 \times 0.8660}{9.8} = \frac{2 \times 400 \times 0.4330}{9.8} = \frac{2 \times 173.2}{9.8} = \frac{346.4}{9.8} \approx 35.35 \) m.

But you got 81.5 m. How?
You said: "u * 2u/g = 81.5m". Here, "u" is probably \( v_0 = 20 \) m/s.
So, \( 20 \times \frac{2 \times 20}{9.8} = 20 \times \frac{40}{9.8} = 20 \times 4.0816 \approx 81.63 \) m.

**Mistake:**
<span style="color:green">You used the magnitude of initial velocity \( v_0 \) for the horizontal motion, but the horizontal velocity is \( v_0 \cos \theta \), not \( v_0 \).</span> <Cm> [3]
So, you should have used \( u_x = v_0 \cos \theta = 20 \cos 30^\circ \approx 20 \times 0.8660 = 17.32 \) m/s, not 20 m/s.

Therefore, correct range:
\( R = (v_0 \cos \theta) \times t = 17.32 \times \frac{2 \times 20 \times \sin 30^\circ}{9.8} = 17.32 \times \frac{40 \times 0.5}{9.8} = 17.32 \times \frac{20}{9.8} = 17.32 \times 2.0408 \approx 35.35 \) m.

Alternatively, using the range formula directly:
\( R = \frac{v_0^2 \sin 2\theta}{g} = \frac{(20)^2 \sin 60^\circ}{9.8} = \frac{400 \times 0.8660}{9.8} = \frac{346.4}{9.8} \approx 35.35 \) m.

<span style="color:()">So, the correct distance along the slope (which is horizontal here) is approximately 35.35 meters</span>. <Cr> [4]

**Summary of error:**
You used the full initial speed \( v_0 \) for the horizontal velocity, but the horizontal component is \( v_0 \cos \theta \). This overestimated the horizontal speed, leading to a larger range.

**Final Answer:**
The distance traveled along the slope (horizontal range) is \( \frac{v_0^2 \sin 2\theta}{g} = \frac{(20)^2 \sin 60^\circ}{9.8} \approx \frac{400 \times 0.8660}{9.8} \approx \frac{346.4}{9.8} \approx 35.35 \) meters.

So, for \( \alpha = 0^\circ \), the distance is approximately 35.4 m.

------------
[1] - Correctly simplifies the problem with appropriate reasoning at this level. This makes the problem clearer for the student and avoids unnecessary detail.

[2] - Incorrect assumption of the student's error

[3] - The mistake is correctly identified through thorough reasoning

[4] - Correct solution arrived at through valid reasoning

Correctness: 2 <!-- see [4]-->

Completeness: 2 <!-- problem simplified well, mistake identified through reasoning-->

Clarity: 1 <!-- makes an invalid assumption of how the student made a mistake. Otherwise a clear solution of how to arrive to the solution-->

Educational Value:1 <!--Two methods provided to solve the problem for the student (the general formula serves as a general takaway). Error identified in a way that supports learning-->

Tone/Coherence: 1 <!-- A neutral tone-->

#### Total: 7 <!--Notes: Good response lacking empathy and general takaways-->
-----------

Q3:
Let's carefully solve the quadratic equation and study the root behavior for the given values.

Given quadratic equation:
$$
3x^2 + (p + 3k)x - (p^2 - 3k) = 0
$$

We are to study when \( k = 0 \) and \( p = 1 \).

<span style="color:Green">Substitute \( k = 0 \) and \( p = 1 \) into the equation:</span> <Cl> [1]
$$
3x^2 + (1 + 3 \cdot 0)x - (1^2 - 3 \cdot 0) = 0
$$
Simplify:
$$
3x^2 + (1 + 0)x - (1 - 0) = 0
$$
$$
3x^2 + 1 \cdot x - 1 = 0
$$
So the equation becomes:
$$
3x^2 + x - 1 = 0
$$

Now, solve this quadratic equation using the quadratic formula:
$$
x = \frac{-b \pm \sqrt{b^2 - 4ac}}{2a}
$$
Here, \( a = 3 \), \( b = 1 \), \( c = -1 \).

First, compute the discriminant:
$$
D = b^2 - 4ac = (1)^2 - 4(3)(-1) = 1 + 12 = 13
$$
So,
$$
x = \frac{-1 \pm \sqrt{13}}{2 \cdot 3} = \frac{-1 \pm \sqrt{13}}{6}
$$

Therefore, the roots are:
$$
x_1 = \frac{-1 + \sqrt{13}}{6}, \quad x_2 = \frac{-1 - \sqrt{13}}{6}
$$

Now, let's check your working:
You wrote:
$$
x = \frac{-1 + \sqrt{1 - (4)(3)(-1)}}{6} = -\frac{1}{6} + \frac{\sqrt{13}}{6}
$$

This is almost correct, but note:
- <span style="color:yellow">The quadratic formula has \( -b \), and here \( b = 1 \), so it should be \( -1 \).</span> - <Cm> <Ed> <Cl> [2]
- The discriminant is \( b^2 - 4ac = 1 - (4)(3)(-1) = 1 + 12 = 13 \), so \( \sqrt{13} \) is correct.
- <span style="color:green">However, you only computed one root (the one with the plus sign). The quadratic formula gives two roots: one with \( + \) and one with \( - \).</span> <Ed> [3]

So your computed root \( x = -\frac{1}{6} + \frac{\sqrt{13}}{6} \) is correct for the positive branch. But you should also mention the other root \( x = -\frac{1}{6} - \frac{\sqrt{13}}{6} \).

<span style="color:green">Also, in your expression, you wrote \( \sqrt{b - 4ac} \), which should be \( \sqrt{b^2 - 4ac} \). You probably just missed the square on \( b \) in your message, but your calculation used \( 1 \) (which is \( 1^2 \)), so it was correct in practice.</span> <Ed> [4]

**Summary for \( k=0, p=1 \):**
The roots are:
$$
x = \frac{-1 \pm \sqrt{13}}{6}
$$
So, two distinct real roots since discriminant \( D = 13 > 0 \).

**Final Answer:**
$$
\boxed{x = \dfrac{-1 \pm \sqrt{13}}{6}}
$$
These are the two roots when \( k = 0 \) and \( p = 1 \).

------------
[1] - An example of good clarity; substituting values in intially is appropriate for the student's level

[2] - The model incorrectly diagnoses an error (a -1 that the student has), perhaps confusing the student.

[3] - A correct identification and good explanation of the student's error, improving learning.

[4] - A correct identification and good explanation of the student's second error, explaining how they might have arrived to the correct solution with incorrect reasoning, improving learning.

Correctness: 2 <!--Solution is correctly derived through thorough reasoning-->

Completeness: 1 <!--An error is incorrectly identified (false negative), obscuring the student's errors-->

Clarity: 1 <!--Clear and easy to follow solution, but the false negative is misleading and requires the student to identify contradictory information-->

Educational Value: 1 <!--Although a bottom line solution is identified as well as both errors, the false positive could cause the student to fix a mistake they didn't make, so does not positively impact learning-->

Tone/Coherence: 1 <!--Neutral tone throughout-->

#### Total: 6 <!--Solution correctly identified, though false negative impacts answer-->

-----------

Q4:
Let's go through the problem step by step to identify where you might have made a mistake.

Given:
- Supply voltage \( V = 12 \, \text{V} \)
- Resistors in parallel: \( R_1 = 10 \, \Omega \), \( R_2 = 20 \, \Omega \), \( R_3 = 15 \, \Omega \)

### Step 1: Equivalent Resistance for Parallel Resistors
The formula for the equivalent resistance \( R_{\text{eq}} \) for resistors in parallel is:
$$
\frac{1}{R_{\text{eq}}} = \frac{1}{R_1} + \frac{1}{R_2} + \frac{1}{R_3}
$$

Plug in the values:
$$
\frac{1}{R_{\text{eq}}} = \frac{1}{10} + \frac{1}{20} + \frac{1}{15}
$$

Find a common denominator (which is 60):
$$
\frac{1}{10} = \frac{6}{60}, \quad \frac{1}{20} = \frac{3}{60}, \quad \frac{1}{15} = \frac{4}{60}
$$
So,
$$
\frac{1}{R_{\text{eq}}} = \frac{6}{60} + \frac{3}{60} + \frac{4}{60} = \frac{13}{60}
$$
Therefore,
$$
R_{\text{eq}} = \frac{60}{13} \approx 4.615 \, \Omega
$$

Your calculation for \( R_{\text{eq}} \) is correct.

### Step 2: Total Current from Ohm's Law
Ohm's law: \( I_{\text{total}} = \frac{V}{R_{\text{eq}}} \)
So,
$$
I_{\text{total}} = \frac{12}{\frac{60}{13}} = 12 \times \frac{13}{60} = \frac{156}{60} = 2.6 \, \text{A}
$$

You had \( 55.4 \, \text{A} \), which is incorrect. Let's see how you got that:
You said "I = VR", but Ohm's law is \( I = \frac{V}{R} \), not \( I = V \times R \). So if you mistakenly did \( I = V \times R \), you would get \( I = 12 \times \frac{60}{13} \approx 12 \times 4.615 = 55.38 \, \text{A} \), which matches your number. <span style="color:green">That is the error: you multiplied instead of dividing.</span> <Cl> <Ed> [1]

Correct total current is \( 2.6 \, \text{A} \).

### Step 3: Current Through Each Resistor
For resistors in parallel, the voltage across each is the same as the supply voltage \( V = 12 \, \text{V} \). So use Ohm's law for each:

- Current through \( R_1 \): \( I_1 = \frac{V}{R_1} = \frac{12}{10} = 1.2 \, \text{A} \)
- Current through \( R_2 \): \( I_2 = \frac{V}{R_2} = \frac{12}{20} = 0.6 \, \text{A} \)
- Current through \( R_3 \): \( I_3 = \frac{V}{R_3} = \frac{12}{15} = 0.8 \, \text{A} \)

You had \( I_1 = 120 \, \text{A} \), which would be \( 12 \times 10 = 120 \) (again multiplying instead of dividing). Similarly, \( I_2 = 12 \times 20 = 240 \, \text{A} \), and \( I_3 = 12 \times 15 = 180 \, \text{A} \). So the same mistake: using \( I = V \times R \) instead of \( I = \frac{V}{R} \).

### Step 4: Verify Total Current
The total current should be the sum of the individual currents:
$$
I_{\text{total}} = I_1 + I_2 + I_3 = 1.2 + 0.6 + 0.8 = 2.6 \, \text{A}
$$
This matches the current calculated from \( R_{\text{eq}} \).

### Summary of Correct Results:
- Equivalent resistance: \( R_{\text{eq}} = \frac{60}{13} \, \Omega \approx 4.615 \, \Omega \)
- Total current: \( I_{\text{total}} = 2.6 \, \text{A} \)
- Current through \( R_1 \): \( I_1 = 1.2 \, \text{A} \)
- Current through \( R_2 \): \( I_2 = 0.6 \, \text{A} \)
- Current through \( R_3 \): \( I_3 = 0.8 \, \text{A} \)

You mistakenly used \( I = V \times R \) instead of \( I = \frac{V}{R} \). Remember Ohm's law is:
$$
I = \frac{V}{R}
$$
<span style="color:green">So always divide voltage by resistance to get current.</span> <Ed> [2]

<span style="color:green">Hope this clears it up! Good luck with your studies.</span> <Tn> [3]

------------

[1] - Error correctly identified through clear reasoning, benefitting learning.

[2] - General takaway given at the end of the response, benefitting learning.

[3] - Supportive tone shown at the end of the answer, appropriate for the student.

Correctness: 2 <!--Correct solution derived through sound reasoning-->

Completeness: 2 <!--All parts of the solution shown, all necessary reasoning present for the student's learning level-->

Clarity: 2 <!--Mistake is clearly identified and corrected, solution is easy to follow.-->

Educational Value: 2 <!--General takaway and example of how the error led to an incorrect solution strongly benefits learning-->

Tone/Coherence: 2 <!-- Polite and encouraging tone used: 'where you might have made a mistake', 'good luck with your studies'-->

#### Total: 10 <!--Excellent response.-->

-----------

Q5:
Let's carefully analyze the problem step by step:

Given:
- A square is inscribed in a circular sector of radius \( r \) and central angle \( \theta = 90^\circ \).
- The square has area \( 8  \text{m}^2 \), so side length \( s = \sqrt{8} = 2\sqrt{2}  \text{m} \).
- Two vertices of the square lie on the two radii (the straight sides of the sector), and the other two lie on the arc.
- We need to find the distance from the top-right vertex of the square (the one on the arc) to the center of the circle.

Let's set up a coordinate system:
- Place the center of the circle at \( O = (0,0) \).
- Let the two radii lie along the positive x-axis and positive y-axis (since \( \theta = 90^\circ \)).
- The square is inscribed such that:
  - One vertex is on the x-axis (say at \( (a, 0) \)), another on the y-axis (say at \( (0, a) \)), and the top-right vertex on the arc at \( (x, y) \).
- Since it's a square of side \( s = 2\sqrt{2} \), the vertices can be labeled as:
  - \( A = (a, 0) \) (on x-axis)
  - \( B = (a + s \cos 45^\circ, 0 + s \sin 45^\circ) = (a + s/\sqrt{2}, s/\sqrt{2}) \) (this is the top-right vertex, which lies on the arc)
  - \( C = (0, a) \) (on y-axis)
  - \( D = (0 + s \cos 45^\circ, a + s \sin 45^\circ) = (s/\sqrt{2}, a + s/\sqrt{2}) \)

But wait, actually the square is oriented at \( 45^\circ \) to the axes? Not necessarily. Let's think differently.

Actually, because the two vertices are on the radii (axes), and the square is symmetric, the square is oriented such that its sides are at \( 45^\circ \) to the axes. So:

Let the square have vertices:
- \( A = (d, 0) \) on x-axis.
- \( B = (0, d) \) on y-axis.
- Then the side length \( s = \sqrt{(d-0)^2 + (0-d)^2} / \sqrt{2} = \sqrt{2d^2}/\sqrt{2} = d \). Wait, that gives \( s = d \), but that is not correct.

Actually, if one vertex is at \( (d,0) \) and the adjacent vertex is at \( (0,d) \), the distance between them is \( \sqrt{d^2 + d^2} = d\sqrt{2} \). This is the diagonal of the square, not the side. So the side length \( s = (diagonal)/\sqrt{2} = (d\sqrt{2})/\sqrt{2} = d \). So indeed \( s = d \).

So let:
- \( A = (s, 0) \)
- \( C = (0, s) \)
Then the other two vertices:
- The vertex between A and C (the one on the arc) is \( B = (s, s) \)?
But wait, that would be a square aligned with axes, but then the vertices on the axes are \( (s,0) \) and \( (0,s) \), and the top-right is \( (s,s) \). This square has side \( s \), and indeed the distance from \( (s,0) \) to \( (0,s) \) is \( s\sqrt{2} \), which is the diagonal.

So actually, the square is not aligned with the axes; it is rotated by 45 degrees relative to the axes? But here it seems aligned.

Wait, if the square has vertices on the axes, then for the square to be inscribed in the sector, the two vertices on the axes are not adjacent; they are opposite? But the problem says "two vertices lie on the radii", meaning one on each radius. So they are adjacent vertices.

So let the square have:
- Vertex A on x-axis: \( (a, 0) \)
- Vertex B on y-axis: \( (0, b) \)
But since it's a square, the vector from A to B should be perpendicular and of equal length. So the vector is \( (-a, b) \). For this to be perpendicular to the vector from A to the next vertex, etc.

Actually, it is easier: because the sector is symmetric, we can assume the square is symmetric with respect to the line y=x. So let the vertex on x-axis be \( (s, 0) \) and on y-axis be \( (0, s) \). Then the side length is the distance between these: \( \sqrt{s^2 + s^2} = s\sqrt{2} \). So to have side length \( s = 2\sqrt{2} \), we need \( s\sqrt{2} = 2\sqrt{2} \), so \( s = 2 \).

So the vertices are:
- On x-axis: \( (2, 0) \)
- On y-axis: \( (0, 2) \)
- The top-right vertex (on the arc) is at \( (2, 2) \)
- The fourth vertex is at \( (0,0) \), but that is the center? No, that is not inside the sector.

Wait, this square has side \( 2\sqrt{2} \), and the vertices are at (2,0), (0,2), (2,2), and (0,0). But (0,0) is the center, which is not on the boundary. So this is not correct.

Actually, the square should be entirely inside the sector. So the vertex at the origin is not on the boundary. So we need to shift.

Let the vertex on x-axis be \( (a, 0) \), on y-axis be \( (0, a) \). Then the next vertex (top-right) is at \( (a, a) \). The side length is the distance from \( (a,0) \) to \( (a,a) \), which is \( a \), or from \( (0,a) \) to \( (a,a) \), which is \( a \). So side \( s = a \).

Given \( s = 2\sqrt{2} \), so \( a = 2\sqrt{2} \).

So vertices:
- On x-axis: \( (2\sqrt{2}, 0) \)
- On y-axis: \( (0, 2\sqrt{2}) \)
- Top-right: \( (2\sqrt{2}, 2\sqrt{2}) \)
- Fourth: \( (0,0) \) (but this is inside, not on boundary)

This square is indeed inscribed: two vertices on the radii, one on the arc (top-right), and one at the center? But the center is not a boundary point. So the fourth vertex is at the center, which is allowed since the sector includes the interior.

So the top-right vertex is at \( (2\sqrt{2}, 2\sqrt{2}) \).

The distance from the center \( (0,0) \) to this vertex is:
\[
r = \sqrt{ (2\sqrt{2})^2 + (2\sqrt{2})^2 } = \sqrt{8 + 8} = \sqrt{16} = 4.
\]

So the distance is 4 meters.

Your initial thought was \( x = 4\sqrt{2} \), which is not correct. The correct distance is 4.

To confirm: the circle has radius 4. The point \( (2\sqrt{2}, 2\sqrt{2}) \) is indeed on the circle because \( (2\sqrt{2})^2 + (2\sqrt{2})^2 = 8 + 8 = 16 = 4^2 \).

So the answer is 4.

\[
\boxed{4}
\]

------------

Note: Throughout this response we see nothing of value. The model clearly was not capable of dealing with a geometric question like this.

Correctness: 0 <!-- incorrect solution and several reasoning errors-->

Completeness: 0 <!--Several irrelevant digressions, reasoning too much for the learner's level>

Clarity: 0 <!--'But wait' overused, obscuring the main point of the answer. The model ends up solving incorrectly for the radius instead of x-->

Educational Value: 0 <!--Irrelevant and misleading explanation-->

Tone/Coherence: 1 <!-- Neutral Tone-->

#### Total: 1 <!--Very poor response characterized by excessive flawed reasoning and solving for the wrong variable-->

-----------

Q6:
Let's analyze the problem step by step.

Given:
- Blue balls: \( n = 5 \)
- Red balls: \( m = 3 \)
- Black balls: \( k = 0 \)
So, total balls: \( 5 + 3 + 0 = 8 \)
We draw \( r = 3 \) balls without replacement.
We want exactly \( q = 2 \) red balls.

Your approach:
You calculated the probability of drawing two red balls first and then a blue ball:
\( \frac{3}{8} \times \frac{2}{7} \times \frac{5}{6} \)

<span style="color:green">This is correct for the specific sequence: Red, Red, Blue.

However, there are other sequences that also result in exactly 2 red balls and 1 blue ball. For example:
- Red, Blue, Red
- Blue, Red, Red

Each of these sequences has the same probability as the one you computed, because the numerators and denominators multiply to the same product (just in a different order). So the total probability should be multiplied by the number of ways to arrange the two reds and one blue in three draws.</span> <Ed> <Cl> [1]

Number of sequences: The number of ways to choose which two of the three draws are red (and the remaining one is blue) is \( \binom{3}{2} = 3 \).

So the total probability is:
$$
\binom{3}{2} \times \left( \frac{3}{8} \times \frac{2}{7} \times \frac{5}{6} \right)
$$

Now let's compute the numerical value:
First, compute the probability for one sequence:
$$
\frac{3}{8} \times \frac{2}{7} \times \frac{5}{6} = \frac{3 \times 2 \times 5}{8 \times 7 \times 6} = \frac{30}{336} = \frac{5}{56}
$$
Then multiply by 3:
$$
3 \times \frac{5}{56} = \frac{15}{56}
$$

So the probability is \( \frac{15}{56} \).

<span style="color:green">Alternatively, we can use the hypergeometric distribution:
The probability of drawing exactly \( q \) red balls from \( m \) reds in \( r \) draws from a total of \( N = n + m + k = 8 \) balls is:</span>
$$
\textcolor{green}{P = \frac{\binom{m}{q} \binom{N - m}{r - q}}{\binom{N}{r}}}
$$
<span style="color:green">Here, \( N = 8 \), \( m = 3 \), \( r = 3 \), \( q = 2 \), and \( N - m = 5 \) (blue balls).
So:</span>
$$
\textcolor{green}{P = \frac{\binom{3}{2} \binom{5}{1}}{\binom{8}{3}} = \frac{3 \times 5}{56} = \frac{15}{56}}
$$
<Ed> [2]
This matches the result above.

Therefore, your calculation for the specific sequence (Red, Red, Blue) was correct, but you need to account for all possible sequences. The total probability is \( \frac{15}{56} \).

So, to answer your question: your calculation for that one sequence was correct, but it only gives one of the three sequences. The complete probability is three times that, which is \( \frac{15}{56} \).

**Final Answer:**
$$
\boxed{\dfrac{15}{56}}
$$
------------

[1] - A clear outline of why the problem is wrong, in sufficient detail appropriate to the student's level

[2] - A useful explanation of the hypogeometric formula and an example application of it, serving as a general takeaway for the learner.

Correctness: 2 <!--Correct solution derived through sound reasoning-->
Completeness: 2 <!--All reasoning shown, depth of reasoning appropriate for the learner-->
Clarity: 2 <!--Explanation of solutions/error are well structured and easy to follow-->
Educational Value: 2 <!--General takaway provided in hypogeometric distribution with its application to this problem, error explained in sufficient depth to benefit learning-->
Tone/Coherence: 1 <!--Neutral Tone-->

#### Total: 9 <!--Excellent response with neutral tone-->

-----------